AesopTest/Unfold.lean
@@ -20,8 +20,46 @@ abbrev WalkingCospan : Type := WidePullbackShape Empty Empty
 @[aesop norm destruct]
 def WalkingCospan_elim : WalkingCospan → Sum Empty Empty := id
 
+/--
+info: Try this:
+  unfold WalkingCospan at h
+  unfold WidePullbackShape at h
+  cases h with
+  | inl val =>
+    have fwd : False := Aesop.BuiltinRules.empty_false val
+    clear val
+    simp_all only
+  | inr val_1 =>
+    have fwd : False := Aesop.BuiltinRules.empty_false val_1
+    clear val_1
+    simp_all only
+-/
+#guard_msgs in
 example (h : WalkingCospan) : α := by
-  aesop (add norm unfold [WidePullbackShape, WalkingCospan])
+  aesop? (add norm unfold [WidePullbackShape, WalkingCospan])
 
 example (h : WalkingCospan) : α := by
   aesop (add norm simp [WidePullbackShape, WalkingCospan])
+
+@[aesop norm unfold]
+def Foo := True
+
+@[aesop norm unfold]
+def Bar := False
+
+/--
+info: Try this:
+  unfold Bar Foo
+  unfold Foo at h₁
+  unfold Foo Bar at h₂
+  simp_all only
+  cases h₂ with
+  | inl val =>
+    simp_all only
+    apply PSum.inr
+    simp_all only
+  | inr val_1 => simp_all only
+-/
+#guard_msgs in
+example (h₁ : Foo) (h₂ : PSum Foo Bar) : PSum Bar Foo := by
+  aesop?
